

1. Conv or Div?

$$(i) \sum_{n=1}^{\infty} (-1)^{n-1} e^{-n/3}$$

$$(ii) \sum_{n=1}^{\infty} (-1)^n \frac{n^2}{n^3+4}$$

$$(iii) \sum_{n=1}^{\infty} \frac{(-1)^{n+1}}{\ln(n+2)}$$

Soln Notice that (i) - (iii) are Alternating Series.

(i) Let  $b_n = e^{-n/3}$ . Notice that  $b_n = e^{-n/3} > 0$

$$\bullet b_{n+1} = e^{-(n+1)/3} \leq b_n = e^{-n/3} \text{ for all } n$$

$$b_n > 0$$

$$b_{n+1} \leq b_n \forall n$$

Why? Let  $f(x) = e^{-x/3}$ . Then  $f'(x) = e^{-x/3} \cdot (-\frac{1}{3}) < 0 \forall x$ , so

we have that  $f(x)$  is decreasing  $\forall x$ .

$$\bullet \lim_{n \rightarrow \infty} b_n = \lim_{n \rightarrow \infty} e^{-n/3} = 0.$$

$$\lim_{n \rightarrow \infty} b_n = 0$$

Hence we may apply the Alternating Series Test (AST) to conclude that (i) is CONVERGENT.

(ii) Clearly,  $b_n = \frac{n^2}{n^3+4}$  for  $n \geq 1$ .

$\bullet$  Let  $f(x) = \frac{x^2}{x^3+4}$ . Then  $f'(x) < 0$

$$\Leftrightarrow \frac{2x(x^3+4) - x^2(3x^2)}{(x^3+4)^2} \leq 0$$

$$\Leftrightarrow \frac{x(2x^3+8-3x^3)}{(x^3+4)^2} \leq 0$$

$$\Leftrightarrow x(8-x^3) \leq 0$$

$$\Leftrightarrow x \leq 0 \quad \text{or} \quad 8 - x^3 \leq 0$$

$$8 \leq x^3$$

$$2 \leq x$$

So,  $b_{n+1} \leq b_n$  whenever  $n \geq 2$ .

• Soln Continued

•  $\lim_{n \rightarrow \infty} b_n = \lim_{n \rightarrow \infty} \frac{n^2}{n^3 + 4} = 0.$

$\deg(\text{num})$   
 $< \deg(\text{denom})$

Hence, we may conclude (ii) is CONVERGENT by AST since  $b_n$  satisfies

•  $b_n > 0$

•  $b_{n+1} \leq b_n \quad \forall n \geq 2$

•  $\lim_{n \rightarrow \infty} b_n = 0$

iii) Let  $b_n = \frac{1}{\ln(n+2)}$ . Again, clearly  $b_n > 0$ .

• Let  $f(x) = \frac{1}{\ln(x+2)}$ . Then

$$f'(x) < 0 \Leftrightarrow \frac{-1}{[\ln(x+2)]^2} \cdot \frac{1}{x+2} \cdot 1 = \frac{-1}{(x+2)[\ln(x+2)]^2} < 0$$

$$\Leftrightarrow -\frac{1}{(x+2)} < 0$$

$$\Leftrightarrow x + 2 > 0$$

$$\Leftrightarrow x > -2$$

Hence  $f(x)$  decreasing when  $x > -2$

i.e.  $b_{n+1} \leq b_n$  when  $n > -2$  so  
 $n = 1$  starting is fine!

i.e.  $b_{n+1} \leq b_n \quad \forall n \geq 1$

•  $\lim_{n \rightarrow \infty} b_n = \lim_{n \rightarrow \infty} \frac{1}{\ln(n+2)} = 0.$  B/c  $\ln(n+2) \rightarrow \infty$  as  $n \rightarrow \infty$

Hence we may conclude that (iii) is CONVERGENT by AST.

2. What is the smallest number of terms of the series

$$\sum_{n=1}^{\infty} (-1)^{n+1} \frac{1}{n3^n}$$

that would have to be added in order to estimate its sum with an absolute error that is less than .01?

Soln Note that

- Alternating series with  $b_n > 0$
- Error less than .01 =  $10^{-2} = \frac{1}{100}$ , i.e. Error  $< \frac{1}{100}$ . It is a strict inequality!
- We can show that  $\sum_{n=1}^{\infty} (-1)^{n+1} \frac{1}{n3^n}$  CONVERGES by AST.

$$\rightarrow \text{If } f(x) = \frac{1}{x3^x}, \text{ then } f'(x) = \frac{-1}{(x3^x)^2} \cdot [1 \cdot 3^x + x \cdot 3^x \ln(3)].$$

$$\text{So, } -[3^x + x \cdot 3^x \ln(3)] < 0$$

$$3^x + x \cdot 3^x \ln(3) > 0$$

$$1 + x \ln(3) > 0$$

$$x > \frac{-1}{\ln(3)} \quad \text{We're OK } \forall n \geq 1.$$

$$\rightarrow \lim_{n \rightarrow \infty} b_n = \lim_{n \rightarrow \infty} \frac{1}{n3^n} = 0 \quad \text{since } n3^n \rightarrow \infty \text{ as } n \rightarrow \infty.$$

Since the series  $\sum_{n=1}^{\infty} (-1)^{n+1} \frac{1}{n3^n}$  is convergent by AST, we can use the Alternating Series Estimation Theorem (ASET).

2. Soln Continued

Observe that

$$\sum_{n=1}^{\infty} \frac{(-1)^{n+1}}{n 3^n} = \frac{1}{1 \cdot 3^1} - \frac{1}{2 \cdot 3^2} + \underbrace{\frac{1}{3 \cdot 3^3}}_{\approx 0.012} - \underbrace{\frac{1}{4 \cdot 3^4}}_{\approx 0.003086} + \dots$$

$$\underbrace{\hspace{10em}}_{S_3 = a_1 + a_2 + a_3}$$

$$\underbrace{\hspace{15em}}_{S_4 = a_1 + a_2 + a_3 + a_4}$$

By ASET,  $|R_n| = |\varepsilon - s_n| \leq b_{n+1} < .01$  provided we choose  $n=3$  since

$$b_{3+1} = b_4 = \frac{1}{4 \cdot 3^4} \approx 0.003086 < .01.$$

Other way, solve  $b_{n+1} < .01$  for  $n!$

3. Which of the series are conditionally convergent?

(i)  $\sum_{n=1}^{\infty} \frac{(-1)^n \arctan(n)}{n^2}$

(ii)  $\sum_{n=1}^{\infty} (-1)^{n-1} \frac{n}{\sqrt{n^4+3}}$

(iii)  $\sum_{n=1}^{\infty} \frac{(-1)^{n+1}}{\cos(1/n)}$

Soln From text, page 738:

Defn We say  $\sum a_n$  is conditionally convergent if it is convergent, but not absolutely convergent.

From text, page 737:

Defn We say  $\sum a_n$  is called absolutely convergent if the series of absolute values  $\sum |a_n|$  is convergent.

From text, page 738

Thm (3) If a series  $\sum a_n$  is absolutely convergent, then it is convergent.

(i)  $\sum_{n=1}^{\infty} \left| \frac{(-1)^n \arctan(n)}{n^2} \right| = \sum_{n=1}^{\infty} \frac{\arctan(n)}{n^2}$  b/c  $\frac{\arctan(n)}{n^2} > 0$  for  $n \geq 1$

But,  $\frac{\arctan}{n^2} \leq \frac{\pi}{2} \cdot \frac{1}{n^2}$  and  $\frac{\pi}{2} \sum_{n=1}^{\infty} \frac{1}{n^2}$  converges as a p-series,

hence (i) is absolutely convergent by the Comparison Test.

(ii)  $\sum_{n=1}^{\infty} \left| \frac{(-1)^{n-1} n}{\sqrt{n^4+3}} \right| = \sum_{n=1}^{\infty} \frac{n}{\sqrt{n^4+3}}$ , since  $\frac{n}{\sqrt{n^4+3}} > 0$  for  $n \geq 1$

Note that  $\sqrt{n^4+3} > \sqrt{n^4}$ , but  $\frac{1}{\sqrt{n^4+3}} < \frac{1}{\sqrt{n^4}}$ . So, multiplying by  $n$  yields

$$\frac{n}{\sqrt{n^4+3}} < \frac{n}{\sqrt{n^4}} = \frac{n}{n^2} = \frac{1}{n}$$

for which  $\sum \frac{1}{n}$  is divergent. Therefore, it is not absolutely convergent.

This just means  $\sum |a_n|$  is divergent. Absolute divergence is not a thing!

3. Soln continued.

(ii) We saw that  $\sum_{n=1}^{\infty} \frac{(-1)^{n+1} n}{\sqrt{n^4+3}}$  is not absolutely convergent. Now, let's show decreasing... Let  $f(x) = \frac{x}{\sqrt{x^4+3}}$ . Then

$$f'(x) = \frac{1 \cdot (x^4+3)^{1/2} - x \cdot \frac{1}{2} (x^4+3)^{-1/2} (4x^3)}{x^4+3} < 0$$

$$\Leftrightarrow 2(x^4+3)^{1/2} - 4x^4(x^4+3)^{-1/2} < 0 \quad (\text{After multiplying by } 2)$$

$$\Leftrightarrow (x^4+3)^{-1/2} [2(x^4+3) - 4x^4] < 0$$

$$\Leftrightarrow -2x^4 + 6 < 0$$

$$\Leftrightarrow \underbrace{1.31607}_{\text{Take 2.}} \approx \sqrt[4]{3} < x$$

So  $b_{n+1} < b_n$  for  $n \geq 2$

$$\text{and } \lim_{n \rightarrow \infty} b_n = \lim_{n \rightarrow \infty} \frac{n}{\sqrt{n^4+3}} = \lim_{n \rightarrow \infty} \frac{n}{\sqrt{n^4}} = \lim_{n \rightarrow \infty} \frac{1}{n} = 0$$

Hence, by AST, we have convergence. So, conditionally convergent.

$$(iii) \sum_{n=1}^{\infty} \left| \frac{(-1)^{n+1}}{\cos(1/n)} \right| = \sum_{n=1}^{\infty} \frac{1}{|\cos(1/n)|}$$

$$\text{But, } \lim_{n \rightarrow \infty} \frac{1}{|\cos(1/n)|} = \lim_{n \rightarrow \infty} \frac{1}{|\cos(0)|} = \lim_{n \rightarrow \infty} \frac{1}{1} = 1 \neq 0$$

$\Rightarrow$  By Divergence Test that  $\sum |a_n|$  is divergent.

Notice that  $b_n = \frac{1}{\cos(1/n)} \rightarrow 1$  as  $n \rightarrow \infty$ . So, same argument as

4. Use the ratio test to determine convergence. (i)  $\sum_{n=1}^{\infty} \frac{(n+3)!}{6^{n-1}}$  (ii)  $\sum_{n=1}^{\infty} \frac{(-1)^n 6^{n+1}}{n^4}$  (iii)  $\sum_{n=1}^{\infty} \frac{n^5 \ln n}{n!}$

Soln Ratio Test

$$\text{If } \lim_{n \rightarrow \infty} \left| \frac{a_{n+1}}{a_n} \right| = L = \begin{cases} < 1 & \text{then } \sum a_n \text{ is absolutely convergent} \\ > 1 \text{ or } = \infty & \text{then } \sum a_n \text{ is divergent} \\ = 1 & \text{then Ratio Test is inconclusive} \end{cases}$$

(i) For simplicity, let  $L = \lim_{n \rightarrow \infty}$ .

$$\begin{aligned} L \left| \frac{a_{n+1}}{a_n} \right| &= L \left| \frac{((n+1)+3)!}{6^{(n+1)-1}} \cdot \frac{6^{n-1}}{(n+3)!} \right| \\ &= L \left| \frac{(n+4)(\cancel{n+3})!}{\cancel{6^n}} \cdot \frac{\cancel{6^n} 6^{-1}}{(\cancel{n+3})!} \right| \quad \text{since } n! = n(n-1)! \\ &= L \left| \frac{1}{6} (n+4) \right| = \infty \Rightarrow \sum a_n \text{ divergent} \end{aligned}$$

$$\begin{aligned} \text{(ii)} \quad L \left| \frac{a_{n+1}}{a_n} \right| &= L \left| \frac{(-1)^{n+1} 6^{(n+1)+1}}{(n+1)^4} \cdot \frac{n^4}{(-1)^n 6^{n+1}} \right| \\ &= L \left| \frac{\cancel{6^{n+1}} \cdot 6}{(n+1)^4} \cdot \frac{n^4}{\cancel{6^{n+1}}} \right| \quad * |(-1)^{n+1}| = |(-1)^n| = 1 \\ &= 6 \cdot L \left| \underbrace{\left( \frac{n}{n+1} \right)^4}_{\frac{n}{n+1} \rightarrow 1 \text{ as } n \rightarrow \infty} \right| = 6 \cdot 1 > 1 \Rightarrow \sum a_n \text{ divergent} \end{aligned}$$

3. Soln Continued

$$(iii) \quad \mathcal{L} \left| \frac{(n+1)^5 \ln(n+1)}{(n+1)!} \cdot \frac{n!}{n^5 \ln(n)} \right|$$

$$= \mathcal{L} \left| \frac{(n+1)^5}{(n+1) \cancel{n!}} \cdot \frac{\cancel{n!}}{n^5} \cdot \frac{\ln(n+1)}{\ln(n)} \right|$$

$$= \underbrace{\mathcal{L} \frac{(n+1)^4}{n^5}} \cdot \underbrace{\mathcal{L} \frac{\ln(n+1)}{\ln(n)}} = 0 < 1 \Rightarrow \sum a_n \text{ is abs convergent}$$

$$\mathcal{L} \frac{n^4}{n^5} = 0$$

as  $n \rightarrow \infty$

$$\stackrel{LH}{=} \mathcal{L} \frac{\frac{1}{n+1}}{\frac{1}{n}} = \mathcal{L} \frac{n}{n+1} = 1$$



5. Consider the series  $\sum_{n=1}^{\infty} \frac{4^n (3n)!}{\underbrace{2 \cdot 6 \cdot 10 \cdots (4n+2)}_{a_n}}$ . Find a simplified expression for  $\frac{a_{n+1}}{a_n}$ .

Soln

$$\frac{a_{n+1}}{a_n} = \frac{4^{n+1} (3(n+1))!}{2 \prod_{i=1}^{n+1} (4i+2)} \cdot \frac{2 \prod_{i=1}^n (4i+2)}{4^n (3n)!}$$

$$= \frac{4(3n+3)(3n+2)(3n+1)}{4(n+1)+2}$$

$$= \frac{4(3n+3)(3n+2)(3n+1)}{4n+6}$$

Key results:

$$\bullet (3(n+1))! = (3n+3)! = (3n+3)((3n+3)-1)!$$

$$\bullet \underset{\substack{\uparrow \\ i=0}}{2} \cdot \underset{\substack{\uparrow \\ i=1}}{6} \cdot \underset{\substack{\uparrow \\ i=2}}{10} \cdots \underset{\substack{\uparrow \\ i=n}}{(4n+2)} = \underbrace{2 \prod_{i=1}^n (4i+2)}_{\text{or use } \prod_{i=0}^n (4i+2)}$$

6. Find the interval of convergence of the following power series.

$$\sum_{n=1}^{\infty} \frac{(x-8)^n}{5^n n}$$

Soln 
$$\lim_{n \rightarrow \infty} \left| \frac{(x-8)^{n+1}}{5^{n+1}(n+1)} \cdot \frac{5^n n}{(x-8)^n} \right| = \lim_{n \rightarrow \infty} \left| \frac{1}{5} \cdot \frac{(x-8)}{1} \cdot \frac{n}{n+1} \right|$$

$$= \frac{1}{5} |x-8|$$

By Ratio Test,  $\lim_{n \rightarrow \infty} \left| \frac{a_{n+1}}{a_n} \right| = L < 1$  says  $\sum a_n$  is <sup>absolutely</sup> convergent.

So,

$$\frac{1}{5} |x-8| < 1$$

$$\Leftrightarrow |x-8| < 5$$

$$* |x| < r \Leftrightarrow -r < x < r$$

$$\Leftrightarrow -5 < x-8 < 5$$

$$\Leftrightarrow 3 < x < 13$$

should also check endpoints.

At  $x=3$ : 
$$\sum_{n=1}^{\infty} \frac{(3-8)^n}{5^n n} = \sum_{n=1}^{\infty} \frac{(-1)^n (5)^n}{5^n n} = \sum_{n=1}^{\infty} \frac{(-1)^n}{n}$$

which converges by AST, i.e.  $b_n = \frac{1}{n}$  has property that

- $b_{n+1} = \frac{1}{n+1} < b_n = \frac{1}{n},$

- $\lim_{n \rightarrow \infty} b_n = \lim_{n \rightarrow \infty} \frac{1}{n} = 0.$

6. Soln Continued

At  $x = 13$ :  $\sum_{n=1}^{\infty} \frac{(13-8)^n}{5^n n} = \sum_{n=1}^{\infty} \frac{5^n}{5^n n} = \sum_{n=1}^{\infty} \frac{1}{n}$  which is the Harmonic series ( $p=1$ ) which diverges!

Thus, the interval of convergence is  $[3, 13)$ .

7. Find the radius of convergence of the following power series.

$$\sum_{n=1}^{\infty} \frac{(7x-8)^n}{n^7}$$

Soln  $\lim_{n \rightarrow \infty} \left| \frac{(7x-8)^{n+1}}{(n+1)^7} \cdot \frac{n^7}{(7x-8)^n} \right| = \lim_{n \rightarrow \infty} \left| (7x-8) \cdot \underbrace{\frac{n^7}{(n+1)^7}}_{\rightarrow 1 \text{ as } n \rightarrow \infty} \right| = |7x-8|$

By the Ratio Test, for convergence (absolute), we require

$$\lim_{n \rightarrow \infty} \left| \frac{a_{n+1}}{a_n} \right| = |7x-8| < 1$$

$$\Leftrightarrow \left| 7\left(x - \frac{8}{7}\right) \right| < 1 \quad \text{Has form } -R < x - a < R$$

$$\Leftrightarrow -\frac{1}{7} < x - \frac{8}{7} < \frac{1}{7}$$

$$\Leftrightarrow -\frac{1}{7} + \frac{8}{7} < x < \frac{1}{7} + \frac{8}{7}$$

$$\Leftrightarrow 1 < x < \frac{9}{7}$$

Now, test endpoints as well.

$$x = 1: \sum_{n=1}^{\infty} \frac{(-1)^n}{n^7} \text{ which converges by AST. } \begin{aligned} &\xrightarrow{b_n = 1/n^7 > 0} b_{n+1} < b_n \\ &\xrightarrow{\lim_{n \rightarrow \infty} b_n = 0} \end{aligned}$$

$$x = \frac{9}{7}: \sum_{n=1}^{\infty} \frac{(1)^n}{n^7} = \sum_{n=1}^{\infty} \frac{1}{n^7} \text{ which is a convergent p-series.}$$